add references to Grammar and Expr

Validator/Derive/Enter.lean
@@ -5,11 +5,11 @@ import Validator.Expr.IfExpr
 
 namespace Enter
 
-def enter (x: Expr α) (res: IfExprs α := []): IfExprs α :=
+def enter (x: Expr μ α) (res: IfExprs μ α := []): IfExprs μ α :=
   match x with
   | Expr.emptyset => res
   | Expr.epsilon => res
-  | Expr.tree pred childrenExpr => (IfExpr.mk pred childrenExpr Expr.emptyset) :: res
+  | Expr.tree pred childRef => (IfExpr.mk pred childRef) :: res
   | Expr.or y z => enter y (enter z res)
   | Expr.concat y z =>
     if Expr.nullable y
@@ -17,18 +17,18 @@ def enter (x: Expr α) (res: IfExprs α := []): IfExprs α :=
     else enter y res
   | Expr.star y => enter y res
 
-def deriveEnter (xs: Exprs α): IfExprs α :=
+def deriveEnter (xs: Exprs μ α): IfExprs μ α :=
   List.flatten (List.map Enter.enter xs)
 
-theorem deriveEnter_nil_is_nil {α: Type u}:
-  @deriveEnter α [] = [] := by
+theorem deriveEnter_nil_is_nil {α: Type u} {μ: Nat}:
+  @deriveEnter μ α [] = [] := by
   unfold deriveEnter
   simp
 
-theorem deriveEnter_cons_is_concat {α: Type u} (x: Expr α) (xs: Exprs α):
+theorem deriveEnter_cons_is_concat {α: Type u} (x: Expr μ α) (xs: Exprs μ α):
   deriveEnter (x::xs) = (deriveEnter [x]) ++ (deriveEnter xs) := by
   unfold deriveEnter
   simp
 
-class DeriveEnter (m: Type -> Type u) (α: outParam Type)  where
-  deriveEnter (xs: Exprs α): m (IfExprs α)
+class DeriveEnter (m: Type -> Type u) (μ: Nat) (α: outParam Type)  where
+  deriveEnter (xs: Exprs μ α): m (IfExprs μ α)
