Validator/Expr/Denote.lean
@@ -1,20 +1,305 @@
+import Validator.Std.List
+
 import Validator.Expr.Expr
 import Validator.Expr.Pred
 import Validator.Expr.Language
 
 namespace Denote
 
-def denote {α: Type} [BEq α] (r: Expr α): Language.Lang α :=
-  match r with
-  | Expr.emptyset => Language.emptyset
-  | Expr.epsilon => Language.emptystr
-  | Expr.tree p childrenExpr => Language.tree (Pred.eval p) (denote childrenExpr)
-  | Expr.or x y => Language.or (denote x) (denote y)
-  | Expr.concat x y => Language.concat (denote x) (denote y)
-  | Expr.star x => Language.star (denote x)
+local elab "simp_sizeOf" : tactic => do
+  Lean.Elab.Tactic.evalTactic (<- `(tactic|
+    simp only [ParseTree.mk.sizeOf_spec, List.cons.sizeOf_spec, List.nil.sizeOf_spec])
+  )
 
-def denote_onlyif {α: Type} [BEq α] (condition: Prop) [dcond: Decidable condition] (x: Expr α):
-  denote (Expr.onlyif condition x) = Language.onlyif condition (denote x) := by
+theorem sizeOf_lex [SizeOf α] [SizeOf β]
+  (x1 x2: α)
+  (y1 y2: β)
+  (hx: x1 = x2 \/ sizeOf x1 < sizeOf x2)
+  (hy: sizeOf y1 < sizeOf y2)
+  :Prod.Lex
+    (fun a₁ a₂ => sizeOf a₁ < sizeOf a₂)
+    (fun a₁ a₂ => sizeOf a₁ < sizeOf a₂)
+    (x1, y1)
+    (x2, y2) := by
+  rw [Prod.lex_def]
+  simp only
+  cases hx
+  · apply Or.inr
+    apply And.intro
+    assumption
+    assumption
+  · apply Or.inl
+    assumption
+
+theorem sizeOf_list_append [SizeOf α] (xs ys: List α):
+  sizeOf xs <= sizeOf (ys ++ xs) := by
+  induction ys with
+  | nil =>
+    simp only [List.nil_append, le_refl]
+  | cons y ys ih =>
+    simp +arith only [List.cons_append, List.cons.sizeOf_spec]
+    omega
+
+theorem lt_plus (x y z: Nat):
+  y < z -> x + y < x + z := by
+  simp
+
+theorem sizeOf_list_cons [SizeOf α] (xs ys: List α):
+  sizeOf xs < sizeOf (y::ys ++ xs) := by
+  induction ys with
+  | nil =>
+    simp +arith only [List.cons_append, List.cons.sizeOf_spec]
+    simp only [List.nil_append, le_add_iff_nonneg_left, zero_le]
+  | cons y ys ih =>
+    simp only [List.cons_append] at *
+    simp only [List.cons.sizeOf_spec] at *
+    omega
+
+theorem split_zero_right: (List.splitAt 0 xs).2 = xs := by
+  simp
+
+theorem exists_drop (n: Nat) (xs: List α): ∃ ys, xs = ys ++ (List.drop n xs) := by
+  induction n with
+  | zero =>
+    exists []
+  | succ n ih =>
+    cases ih with
+    | intro ys ih =>
+      cases xs with
+      | nil =>
+        simp at *
+      | cons x xs =>
+        simp only [List.drop_succ_cons]
+        exists (x::List.take n xs)
+        simp
+
+theorem sizeOf_take (xs: ParseForest α):
+  List.take n xs = xs \/ sizeOf (List.take n xs) < sizeOf xs := by
+  simp
+  by_cases (List.length xs > n)
+  case pos h =>
+    apply Or.inr
+    induction n generalizing xs with
+    | zero =>
+      simp only [List.take]
+      simp_sizeOf
+      cases xs with
+      | nil =>
+        simp at h
+      | cons x xs =>
+        simp_sizeOf
+        cases x
+        simp_sizeOf
+        omega
+    | succ n' ih =>
+      cases xs with
+      | nil =>
+        simp at h
+      | cons x xs =>
+        simp only [List.take]
+        simp_sizeOf
+        simp at h
+        apply lt_plus
+        apply ih
+        exact h
+  case neg h =>
+    simp at h
+    apply Or.inl
+    assumption
+
+def denote {α: Type} [BEq α] (g: Expr.Grammar μ α) (x: Expr μ α) (as: ParseForest α): Prop :=
+  match x with
+  | Expr.emptyset => False
+  | Expr.epsilon => as = []
+  | Expr.tree p childref => -- (tree (Pred.eval p) (denote g (g.lookup childref))) xs
+    match as with
+    | [ParseTree.mk label children] => Pred.eval p label /\ (denote g (g.lookup childref) children)
+    | _ => False
+  | Expr.or y z => (denote g y as) \/ (denote g z as)
+  | Expr.concat y z => ∃ n,
+      denote g y (List.take n as) /\ denote g z (List.drop n as)
+  | Expr.star y =>
+    match as with
+    | [] => True
+    | (a::as) => ∃ n,
+        (denote g y (a::(List.take n as)))
+        /\ (denote g (Expr.star y) (List.drop n as))
+  termination_by (as, x)
+  decreasing_by
+  · apply Prod.Lex.left
+    simp +arith only [List.cons.sizeOf_spec, ParseTree.mk.sizeOf_spec, sizeOf_default, add_zero,
+      List.nil.sizeOf_spec]
+  · apply Prod.Lex.right
+    simp +arith only [Expr.or.sizeOf_spec]
+  · apply Prod.Lex.right
+    simp +arith only [Expr.or.sizeOf_spec]
+  · apply sizeOf_lex
+    · apply sizeOf_take
+    · simp [Expr.concat.sizeOf_spec]
+      omega
+  · have h := exists_drop (xs := as) (n := n)
+    cases h with
+    | intro ys h =>
+    nth_rewrite 2 [h]
+    cases ys with
+    | nil =>
+      apply Prod.Lex.right
+      simp +arith only [Expr.concat.sizeOf_spec]
+    | cons y ys =>
+      apply Prod.Lex.left
+      apply sizeOf_list_cons
+  · nth_rw 1 [Prod.lex_def]
+    simp only [List.cons.sizeOf_spec, add_lt_add_iff_left, List.cons.injEq,
+      true_and, Expr.star.sizeOf_spec, lt_add_iff_pos_left, zero_lt_one, and_true]
+    apply Or.symm
+    apply sizeOf_take
+  · apply Prod.Lex.left
+    have h := exists_drop (xs := as) (n := n)
+    cases h with
+    | intro ys h =>
+    nth_rewrite 2 [h]
+    apply sizeOf_list_cons
+
+theorem denote_emptyset {α: Type} [BEq α] {g: Expr.Grammar μ α}:
+  denote g Expr.emptyset = Language.emptyset := by
+  unfold Language.emptyset
+  funext
+  simp [denote]
+
+theorem denote_epsilon {α: Type} [BEq α] {g: Expr.Grammar μ α}:
+  denote g Expr.epsilon = Language.emptystr := by
+  unfold Language.emptystr
+  funext
+  simp [denote]
+
+theorem denote_tree {α: Type} [BEq α] {g: Expr.Grammar μ α} (p: Pred α):
+  denote g (Expr.tree p r) = Language.tree (Pred.eval p) (denote g (g.lookup r)) := by
+  unfold Language.tree
+  funext xs
+  simp
+  apply Iff.intro
+  case mp =>
+    intro h
+    cases xs with
+    | nil =>
+      simp [denote] at h
+    | cons x xs =>
+      cases xs with
+      | nil =>
+        cases x with
+        | mk label children =>
+          exists label
+          exists children
+          apply And.intro rfl
+          simp [denote] at h
+          assumption
+      | cons x2 xs =>
+        simp [denote] at h
+  case mpr =>
+    intro h
+    cases h with
+    | intro label h =>
+    cases h with
+    | intro children h =>
+    cases h with
+    | intro hxs h =>
+    rw [hxs]
+    simp [denote]
+    assumption
+
+theorem denote_or {α: Type} [BEq α] {g: Expr.Grammar μ α} (x y: Expr μ α):
+  denote g (Expr.or x y) = Language.or (denote g x) (denote g y) := by
+  unfold Language.or
+  funext xs
+  simp [denote]
+
+theorem denote_concat {α: Type} [BEq α] {g: Expr.Grammar μ α} (x y: Expr μ α):
+  denote g (Expr.concat x y) = Language.concat (denote g x) (denote g y) := by
+  unfold Language.concat
+  funext xs
+  simp [denote]
+  apply Iff.intro
+  case mp =>
+    intro h
+    cases h with
+    | intro n h =>
+    cases h with
+    | intro hx hy =>
+    exists (List.take n xs)
+    apply And.intro hx
+    exists (List.drop n xs)
+    apply And.intro hy
+    simp
+  case mpr =>
+    intro h
+    cases h with
+    | intro xs h =>
+    cases h with
+    | intro hx h =>
+    cases h with
+    | intro ys h =>
+    cases h with
+    | intro hy hxsys =>
+    rw [hxsys]
+    exists List.length xs
+    simp
+    apply And.intro hx hy
+
+theorem denote_star' {α: Type} [BEq α] {g: Expr.Grammar μ α} (y: Expr μ α) (as: ParseForest α):
+  denote g (Expr.star y) as <-> Language.star (denote g y) as := by
+  apply Iff.intro
+  case mp =>
+    intro h
+    cases as with
+    | nil =>
+      apply Language.star.zero
+    | cons a as =>
+      simp [denote] at h
+      cases h with
+      | intro n h =>
+      cases h with
+      | intro h1 h2 =>
+      apply Language.star.more a (List.take n as) (List.drop n as)
+      · simp
+      · exact h1
+      · rw [<- denote_star']
+        exact h2
+  case mpr =>
+    intro h
+    cases as with
+    | nil =>
+      simp [denote]
+    | cons a as =>
+      simp [denote]
+      cases h with
+      | more a1 as1 as2 _ hxy h1 h2  =>
+        cases hxy
+        exists List.length as1
+        simp
+        apply And.intro h1
+        rw [denote_star']
+        exact h2
+  termination_by as
+  decreasing_by
+    · have h' := exists_drop n tail
+      cases h' with
+      | intro ys h' =>
+      nth_rewrite 2 [h']
+      simp_sizeOf
+      have h'' := sizeOf_list_append (List.drop n tail) ys
+      omega
+    · rename_i j1 j2 j3 j4 j5 j6 j7 j8 j9 _j10
+      cases j4
+      rw [<- j6]
+      apply sizeOf_list_cons
+
+theorem denote_star {α: Type} [BEq α] {g: Expr.Grammar μ α} (y: Expr μ α):
+  denote g (Expr.star y) = Language.star (denote g y) := by
+  funext xs
+  rw [denote_star']
+
+def denote_onlyif {α: Type} [BEq α] (condition: Prop) [dcond: Decidable condition] (g: Expr.Grammar μ α) (x: Expr μ α):
+  denote g (Expr.onlyif condition x) = Language.onlyif condition (denote g x) := by
   unfold Language.onlyif
   unfold Expr.onlyif
   funext xs
@@ -26,45 +311,44 @@ def denote_onlyif {α: Type} [BEq α] (condition: Prop) [dcond: Decidable condit
   case neg hc =>
     simp only [eq_iff_iff]
     rw [denote]
-    rw [Language.emptyset]
     simp only [false_iff, not_and]
     intro hc'
     contradiction
 
-theorem null_commutes {α: Type} [BEq α] (x: Expr α):
-  ((Expr.nullable x) = true) = Language.null (denote x) := by
+theorem null_commutes {α: Type} [BEq α] (g: Expr.Grammar μ α) (x: Expr μ α):
+  ((Expr.nullable x) = true) = Language.null (denote g x) := by
   induction x with
   | emptyset =>
-    unfold denote
+    rw [denote_emptyset]
     rw [Language.null_emptyset]
     unfold Expr.nullable
     apply Bool.false_eq_true
   | epsilon =>
-    unfold denote
+    rw [denote_epsilon]
     rw [Language.null_emptystr]
     unfold Expr.nullable
     simp only
   | tree p children =>
-    unfold denote
+    rw [denote_tree]
     rw [Language.null_tree]
     unfold Expr.nullable
     apply Bool.false_eq_true
   | or p q ihp ihq =>
-    unfold denote
+    rw [denote_or]
     rw [Language.null_or]
     unfold Expr.nullable
     rw [<- ihp]
     rw [<- ihq]
     rw [Bool.or_eq_true]
   | concat p q ihp ihq =>
-    unfold denote
+    rw [denote_concat]
     rw [Language.null_concat]
     unfold Expr.nullable
     rw [<- ihp]
     rw [<- ihq]
     rw [Bool.and_eq_true]
   | star r ih =>
-    unfold denote
+    rw [denote_star]
     rw [Language.null_star]
     unfold Expr.nullable
     simp only
