Validator/Expr/Expr.lean
@@ -1,29 +1,31 @@
 import Validator.Std.Linter.DetectClassical
 
+import Mathlib.Tactic.RewriteSearch
+
 import Validator.Expr.Pred
 
-inductive Expr α where
+inductive Expr μ α where
   | emptyset
   | epsilon
-  | tree (labelPred: Pred α) (childrenExpr: Expr α)
-  | or (y z: Expr α)
-  | concat (y z: Expr α)
-  | star (y: Expr α)
+  | tree (labelPred: Pred α) (ref: Fin μ)
+  | or (y z: Expr μ α)
+  | concat (y z: Expr μ α)
+  | star (y: Expr μ α)
   deriving DecidableEq, Ord, Repr, Hashable
 
-abbrev Exprs α := List (Expr α)
+abbrev Exprs μ α := List (Expr μ α)
 
-instance [Ord α]: Ord (Expr α) := inferInstance
+instance [Ord α]: Ord (Expr μ α) := inferInstance
 
-instance [Repr α]: Repr (Expr α) := inferInstance
+instance [Repr α]: Repr (Expr μ α) := inferInstance
 
-instance [DecidableEq α]: DecidableEq (Expr α) := inferInstance
+instance [DecidableEq α]: DecidableEq (Expr μ α) := inferInstance
 
-instance [DecidableEq α]: BEq (Expr α) := inferInstance
+instance [DecidableEq α]: BEq (Expr μ α) := inferInstance
 
-instance [Hashable α]: Hashable (Expr α) := inferInstance
+instance [Hashable α]: Hashable (Expr μ α) := inferInstance
 
-def Expr.nullable (x: Expr α): Bool :=
+def Expr.nullable (x: Expr μ α): Bool :=
   match x with
   | Expr.emptyset => false
   | Expr.epsilon => true
@@ -32,17 +34,17 @@ def Expr.nullable (x: Expr α): Bool :=
   | Expr.concat y z => nullable y && nullable z
   | Expr.star _ => true
 
-def Expr.unescapable (x: Expr α): Bool :=
+def Expr.unescapable (x: Expr μ α): Bool :=
   match x with
   | Expr.emptyset => true
   | _ => false
 
 namespace Expr
 
-def onlyif (cond: Prop) [dcond: Decidable cond] (x: Expr α): Expr α :=
+def onlyif (cond: Prop) [dcond: Decidable cond] (x: Expr μ α): Expr μ α :=
   if cond then x else Expr.emptyset
 
-def smartOr (x y: Expr α): Expr α :=
+def smartOr (x y: Expr μ α): Expr μ α :=
   match x with
   | Expr.emptyset => y
   | _ =>
@@ -50,7 +52,7 @@ def smartOr (x y: Expr α): Expr α :=
     | Expr.emptyset => x
     | _ => Expr.or x y
 
-def smartConcat (x y: Expr α): Expr α :=
+def smartConcat (x y: Expr μ α): Expr μ α :=
   match x with
   | Expr.emptyset => Expr.emptyset
   | Expr.epsilon => y
@@ -60,8 +62,171 @@ def smartConcat (x y: Expr α): Expr α :=
     | Expr.epsilon => x
     | _ => Expr.concat x y
 
-def smartStar (x: Expr α): Expr α :=
+def smartStar (x: Expr μ α): Expr μ α :=
   match x with
   | Expr.star _ => x
   | Expr.emptyset => Expr.epsilon
   | _ => Expr.star x
+
+def references (x: Expr μ α): List (Fin μ) :=
+  match x with
+  | Expr.emptyset => []
+  | Expr.epsilon => []
+  | Expr.tree _ r => [r]
+  | Expr.or y z => references y ++ references z
+  | Expr.concat y z => references y ++ references z
+  | Expr.star y => references y
+
+structure Grammar μ α where
+  main: Expr μ α
+  refs: Vector (Expr μ α) (μ - 1)
+
+def Grammar.references (g: Grammar μ α): List (Fin μ) :=
+  List.flatten (List.map Expr.references (g.main :: g.refs.toList))
+
+def Grammar.lookup (g: Grammar μ α) (ref: Fin μ): Expr μ α :=
+  match ref with
+  | Fin.mk 0 _ =>
+    g.main
+  | Fin.mk (m + 1) _ =>
+    Vector.get g.refs (Fin.mk m (by omega))
+
+def Grammar.singleton (x: Expr 1 α): Grammar 1 α :=
+  Grammar.mk x #v[]
+
+def Grammar.lookup0 (g: Grammar μ α): Expr μ α :=
+  g.main
+
+def Grammar.emptyset: Grammar 1 α :=
+  Grammar.mk Expr.emptyset #v[]
+
+def Grammar.epsilon: Grammar 1 α :=
+  Grammar.mk Expr.epsilon #v[]
+
+def Expr.setMaxRef (μ1: Nat) (h: μ1 >= μ0) (x: Expr μ0 α): Expr μ1 α :=
+  match x with
+  | emptyset => Expr.emptyset
+  | epsilon => Expr.epsilon
+  | tree p ref => Expr.tree p (Fin.mk ref.val (by omega))
+  | or y z => Expr.or (Expr.setMaxRef μ1 h y) (Expr.setMaxRef μ1 h z)
+  | concat y z => Expr.concat (Expr.setMaxRef μ1 h y) (Expr.setMaxRef μ1 h z)
+  | star y => Expr.star (Expr.setMaxRef μ1 h y)
+
+def maxref (μold μnew μ: Nat): Nat :=
+  if μold + 1 = μ -- if mold is the maximum ref
+  then
+    max (μ - 1) (μnew + 1) -- then downgrade to m - 1 or upgrade to mnew
+  else
+    (max μ (μnew + 1)) -- otherwise upgrade to mnew
+
+def Expr.rewriteRef (μold μnew: Nat) (x: Expr μ α): Expr (maxref μold μnew μ) α :=
+  match x with
+  | emptyset => Expr.emptyset
+  | epsilon => Expr.epsilon
+  | tree p ref =>
+    if h: ref = μold
+    then Expr.tree p (Fin.mk μnew (by
+      unfold maxref
+      split_ifs
+      · omega
+      · omega
+      ))
+    else Expr.tree p (Fin.mk ref.val (by
+      unfold maxref
+      split_ifs
+      · omega
+      · omega
+      ))
+  | or y z => Expr.or (Expr.rewriteRef μold μnew y) (Expr.rewriteRef μold μnew z)
+  | concat y z => Expr.concat (Expr.rewriteRef μold μnew y) (Expr.rewriteRef μold μnew z)
+  | star y => Expr.star (Expr.rewriteRef μold μnew y)
+
+example :
+  Expr.rewriteRef 2 2
+  ((Expr.tree (Pred.eq 'a') (Fin.mk 2 (by omega))): Expr 3 Char)
+  =
+  ((Expr.tree (Pred.eq 'a') (Fin.mk 2 (by omega))): Expr 3 Char) := by
+  simp only [Expr.rewriteRef, ↓reduceDIte, ↓Char.isValue]
+
+example :
+  Expr.rewriteRef 2 3
+  ((Expr.tree (Pred.eq 'a') (Fin.mk 2 (by omega))): Expr 3 Char)
+  =
+  ((Expr.tree (Pred.eq 'a') (Fin.mk 3 (by omega))): Expr 4 Char) := by
+  simp only [Expr.rewriteRef, ↓reduceDIte, ↓Char.isValue]
+
+example :
+  Expr.rewriteRef 2 5
+  ((Expr.tree (Pred.eq 'a') (Fin.mk 2 (by omega))): Expr 3 Char)
+  =
+  ((Expr.tree (Pred.eq 'a') (Fin.mk 5 (by omega))): Expr 6 Char) := by
+  simp only [Expr.rewriteRef, ↓reduceDIte, ↓Char.isValue]
+
+example :
+  Expr.rewriteRef 2 1
+  ((Expr.tree (Pred.eq 'a') (Fin.mk 2 (by omega))): Expr 3 Char)
+  =
+  ((Expr.tree (Pred.eq 'a') (Fin.mk 1 (by omega))): Expr 2 Char) := by
+  simp only [Expr.rewriteRef, ↓reduceDIte, ↓Char.isValue, Fin.mk_one, Fin.isValue]
+
+example :
+  Expr.rewriteRef 5 2
+  ((Expr.tree (Pred.eq 'a') (Fin.mk 5 (by omega))): Expr 6 Char)
+  =
+  -- We only downgrade by one to 5, since the previous one was erroniously set to 6
+  -- It might be part of a grammar with expressions of higher
+  ((Expr.tree (Pred.eq 'a') (Fin.mk 2 (by omega))): Expr 5 Char) := by
+  simp only [Expr.rewriteRef, ↓reduceDIte, ↓Char.isValue]
+
+def Expr.rewriteIncRef (μold μnew: Nat) (x: Expr μ α): Expr (max μ (μnew + 1)) α :=
+  match x with
+  | emptyset => Expr.emptyset
+  | epsilon => Expr.epsilon
+  | tree p ref =>
+    if h: ref = μold
+    then Expr.tree p (Fin.mk μnew (by omega))
+    else Expr.tree p (Fin.mk ref.val (by omega))
+  | or y z => Expr.or (Expr.rewriteIncRef μold μnew y) (Expr.rewriteIncRef μold μnew z)
+  | concat y z => Expr.concat (Expr.rewriteIncRef μold μnew y) (Expr.rewriteIncRef μold μnew z)
+  | star y => Expr.star (Expr.rewriteIncRef μold μnew y)
+
+def Expr.incRefs (x: Expr μ α): Expr (μ + 1) α :=
+  match x with
+  | emptyset => Expr.emptyset
+  | epsilon => Expr.epsilon
+  | tree p ref => Expr.tree p (Fin.mk (ref.val + 1) (by omega))
+  | or y z => Expr.or (Expr.incRefs y) (Expr.incRefs z)
+  | concat y z => Expr.concat (Expr.incRefs y) (Expr.incRefs z)
+  | star y => Expr.star (Expr.incRefs y)
+
+theorem max_pos {x y: Nat}:
+  x < y -> y = (max x y) := by omega
+
+theorem max_neg {x y: Nat}:
+  ¬ x < y -> x = (max x y) := by omega
+
+theorem lt_ge {x y: Nat}:
+  x < y -> y >= x := by omega
+
+theorem not_lt_ge {x y: Nat}:
+  ¬ x < y -> x >= y := by omega
+
+private def example_grammar: Grammar 2 Char :=
+  Grammar.mk
+    (Expr.or Expr.epsilon (Expr.tree (Pred.eq 'a') 1))
+    #v[Expr.epsilon]
+
+#guard
+  example_grammar.lookup (Fin.mk 0 (by omega))
+  = (Expr.or Expr.epsilon (Expr.tree (Pred.eq 'a') 1))
+
+#guard
+  example_grammar.lookup (Fin.mk 1 (by omega))
+  = Expr.epsilon
+
+def lookup_all (g: Grammar μ α): Exprs μ α :=
+  List.map g.lookup (Grammar.references g)
+
+#guard
+  lookup_all example_grammar
+  = [Expr.epsilon]
