Validator/Learning/ImperativeBasic.lean
@@ -15,7 +15,7 @@ import Validator.Learning.ImperativeLeave
 namespace ImperativeBasic
 
 -- foldLoop is a more readable version of List.foldlM for imperative programmers:
-private def foldLoop (deriv: Exprs α -> ParseTree α -> Except String (Exprs α)) (start: Exprs α) (forest: ParseForest α): Except String (Exprs α) := do
+private def foldLoop (deriv: Exprs μ α -> ParseTree α -> Except String (Exprs μ α)) (start: Exprs μ α) (forest: ParseForest α): Except String (Exprs μ α) := do
   let mut res := start
   for tree in forest do
     match deriv res tree with
@@ -23,7 +23,7 @@ private def foldLoop (deriv: Exprs α -> ParseTree α -> Except String (Exprs α
     | Except.ok r => res := r
   return res
 
-def derive [DecidableEq α] (xs: Exprs α) (tree: ParseTree α): Except String (Exprs α) :=
+def derive [DecidableEq α] (g: Expr.Grammar μ α) (xs: Exprs μ α) (tree: ParseTree α): Except String (Exprs μ α) :=
   -- If all expressions are unescapable, then simply return without look at the input tree.
   -- An example of an unescapable expression is emptyset, since its derivative is always emptyset, no matter the input.
   if List.all xs Expr.unescapable
@@ -33,37 +33,37 @@ def derive [DecidableEq α] (xs: Exprs α) (tree: ParseTree α): Except String (
     match tree with
     | ParseTree.mk label children =>
       -- enters is one of our two new memoizable functions.
-      let ifexprs: IfExprs α := Enter.deriveEnter xs
+      let ifexprs: IfExprs μ α := Enter.deriveEnter xs
       -- childxs = expressions to evaluate on children.
-      let childxs: Exprs α := IfExpr.evals ifexprs label
+      let childxs: Exprs μ α := IfExpr.evals g ifexprs label
       -- dchildxs = derivatives of children. The ' is for the exception it is wrapped in.
       -- see foldLoop for an explanation of what List.foldM does.
-      let dchildxs': Except String (Exprs α) := List.foldlM derive childxs children
+      let dchildxs': Except String (Exprs μ α) := List.foldlM (derive g) childxs children
       match dchildxs' with
       | Except.error err => Except.error err
       | Except.ok dchildxs =>
       -- dxs = derivatives of xs. The ' is for the exception it is wrapped in.
       -- leaves is the other one of our two new memoizable functions.
-      let dxs': Except String (Exprs α) := ImperativeLeave.deriveLeave xs (List.map Expr.nullable dchildxs)
+      let dxs': Except String (Exprs μ α) := ImperativeLeave.deriveLeave xs (List.map Expr.nullable dchildxs)
       match dxs' with
       | Except.error err => Except.error err
       | Except.ok dxs => Except.ok dxs
 
-def derivs [DecidableEq α] (x: Expr α) (forest: ParseForest α): Except String (Expr α) :=
+def derivs [DecidableEq α] (g: Expr.Grammar μ α) (x: Expr μ α) (forest: ParseForest α): Except String (Expr μ α) :=
   -- see foldLoop for an explanation of what List.foldM does.
-  let dxs := List.foldlM derive [x] forest
+  let dxs := List.foldlM (derive g) [x] forest
   match dxs with
   | Except.error err => Except.error err
   | Except.ok [dx] => Except.ok dx
   | Except.ok _ => Except.error "expected one expression"
 
-def validate [DecidableEq α] (x: Expr α) (forest: ParseForest α): Except String Bool :=
-  match derivs x forest with
+def validate [DecidableEq α] (g: Expr.Grammar μ α) (x: Expr μ α) (forest: ParseForest α): Except String Bool :=
+  match derivs g x forest with
   | Except.error err => Except.error err
   | Except.ok x' => Except.ok (Expr.nullable x')
 
-def run [DecidableEq α] (x: Expr α) (t: ParseTree α): Except String Bool :=
-  validate x [t]
+def run [DecidableEq α] (g: Expr.Grammar μ α) (t: ParseTree α): Except String Bool :=
+  validate g g.lookup0 [t]
 
 -- Tests
 -- Lean can use #guard to run these tests at compile time.
@@ -71,55 +71,62 @@ def run [DecidableEq α] (x: Expr α) (t: ParseTree α): Except String Bool :=
 open TokenTree (node)
 
 #guard run
-  Expr.emptyset
+  (Expr.Grammar.singleton Expr.emptyset)
   (node "a" [node "b" [], node "c" [node "d" []]]) =
   Except.ok false
 
 #guard run
-  (Expr.tree (Pred.eq (Token.string "a")) Expr.epsilon)
+  (Expr.Grammar.mk (μ := 2)
+    (Expr.tree (Pred.eq (Token.string "a")) 1)
+    #v[Expr.epsilon]
+  )
   (node "a" []) =
   Except.ok true
 
 #guard run
-  (Expr.tree (Pred.eq (Token.string "a")) Expr.epsilon)
+  (Expr.Grammar.mk (μ := 2)
+    (Expr.tree (Pred.eq (Token.string "a")) 1)
+    #v[Expr.epsilon]
+  )
   (node "a" [node "b" []]) =
   Except.ok false
 
 #guard run
-  (Expr.tree (Pred.eq (Token.string "a"))
-    (Expr.tree (Pred.eq (Token.string "b"))
-      Expr.epsilon
-    )
+  (Expr.Grammar.mk (μ := 3)
+    (Expr.tree (Pred.eq (Token.string "a")) 1)
+    #v[
+      (Expr.tree (Pred.eq (Token.string "b")) 2)
+      , Expr.epsilon
+    ]
   )
-  (node "a" [node "b" []]) =
-  Except.ok true
+  (node "a" [node "b" []])
+  = Except.ok true
 
 #guard run
-  (Expr.tree (Pred.eq (Token.string "a"))
-    (Expr.concat
-      (Expr.tree (Pred.eq (Token.string "b"))
-        Expr.epsilon
+  (Expr.Grammar.mk (μ := 3)
+    (Expr.tree (Pred.eq (Token.string "a")) 1)
+    #v[
+      (Expr.concat
+        (Expr.tree (Pred.eq (Token.string "b")) 2)
+        (Expr.tree (Pred.eq (Token.string "c")) 2)
       )
-      (Expr.tree (Pred.eq (Token.string "c"))
-        Expr.epsilon
-      )
-    )
+      , Expr.epsilon
+    ]
   )
   (node "a" [node "b" [], node "c" []]) =
   Except.ok true
 
 #guard run
-  (Expr.tree (Pred.eq (Token.string "a"))
-    (Expr.concat
-      (Expr.tree (Pred.eq (Token.string "b"))
-        Expr.epsilon
+  (Expr.Grammar.mk (μ := 4)
+    (Expr.tree (Pred.eq (Token.string "a")) 1)
+    #v[
+      (Expr.concat
+        (Expr.tree (Pred.eq (Token.string "b")) 2)
+        (Expr.tree (Pred.eq (Token.string "c")) 3)
       )
-      (Expr.tree (Pred.eq (Token.string "c"))
-        (Expr.tree (Pred.eq (Token.string "d"))
-          Expr.epsilon
-        )
-      )
-    )
+      , Expr.epsilon
+      , (Expr.tree (Pred.eq (Token.string "d")) 2)
+    ]
   )
   (node "a" [node "b" [], node "c" [node "d" []]]) =
   Except.ok true
