Validator/Learning/Parser.lean
@@ -19,167 +19,190 @@ import Validator.Validator.Inst.TreeParserM
 
 namespace Parser
 
-def deriveEnter [DecidableEq α] [ValidateM m α] (xs: Exprs α): m (Exprs α) := do
+def deriveEnter [DecidableEq α] [ValidateM m μ α] (g: Expr.Grammar μ α) (xs: Exprs μ α): m (Exprs μ α) := do
   let enters <- Enter.DeriveEnter.deriveEnter xs
   let token <- Parser.token
-  return IfExpr.evals enters token
+  return IfExpr.evals g enters token
 
-def deriveLeaveM [DecidableEq α] [ValidateM m α] (xs: Exprs α) (cs: Exprs α): m (Exprs α) :=
+def deriveLeaveM [DecidableEq α] [ValidateM m μ α] (xs: Exprs μ α) (cs: Exprs μ α): m (Exprs μ α) :=
   Leave.DeriveLeaveM.deriveLeaveM xs (List.map Expr.nullable cs)
 
-def deriveValue [DecidableEq α] [ValidateM m α] (xs: Exprs α): m (Exprs α) := do
-  deriveEnter xs >>= deriveLeaveM xs
+def deriveValue [DecidableEq α] [ValidateM m μ α] (g: Expr.Grammar μ α) (xs: Exprs μ α): m (Exprs μ α) := do
+  deriveEnter g xs >>= deriveLeaveM xs
 
 -- TODO: Is it possible to have a Parser type that can be proved to be of the correct shape, and have not expection throwing
 -- for example: can you prove that your Parser will never return an Hint.leave after returning a Hint.field.
 -- This class can be called the LawfulParser.
-partial def derive [DecidableEq α] [ValidateM m α] (xs: Exprs α): m (Exprs α) := do
+partial def derive [DecidableEq α] [ValidateM m μ α] (g: Expr.Grammar μ α) (xs: Exprs μ α): m (Exprs μ α) := do
   if List.all xs Expr.unescapable then
     Parser.skip; return xs
   match <- Parser.next with
   | Hint.field =>
-    let childxs <- deriveEnter xs -- derive enter field
+    let childxs <- deriveEnter g xs -- derive enter field
     let dchildxs <-
       match <- Parser.next with
-      | Hint.value => deriveValue childxs -- derive child value
-      | Hint.enter => derive childxs -- derive children, until return from a Hint.leave
+      | Hint.value => deriveValue g childxs -- derive child value
+      | Hint.enter => derive g childxs -- derive children, until return from a Hint.leave
       | hint => throw s!"unexpected {hint}"
     let xsLeave <- deriveLeaveM xs dchildxs -- derive leave field
-    derive xsLeave -- deriv next
-  | Hint.value => deriveValue xs >>= derive -- derive value and then derive next
-  | Hint.enter => derive xs >>= derive -- derive children, until return from a Hint.leave and then derive next
+    derive g xsLeave -- deriv next
+  | Hint.value => deriveValue g xs >>= derive g -- derive value and then derive next
+  | Hint.enter => derive g xs >>= derive g -- derive children, until return from a Hint.leave and then derive next
   | Hint.leave => return xs -- never happens at the top
   | Hint.eof => return xs -- only happens at the top
 
-def validate {m} [DecidableEq α] [ValidateM m α] (x: Expr α): m Bool := do
-  let dxs <- derive [x]
+def validate {m} [DecidableEq α] [ValidateM m μ α] (g: Expr.Grammar μ α) (x: Expr μ α): m Bool := do
+  let dxs <- derive g [x]
   match dxs with
   | [dx] => return Expr.nullable dx
   | _ => throw "expected one expression"
 
-def run [DecidableEq α] (x: Expr α) (t: ParseTree α): Except String Bool :=
-  TreeParserM.run' (validate x) t
+def run [DecidableEq α] (g: Expr.Grammar μ α) (t: ParseTree α): Except String Bool :=
+  TreeParserM.run' (validate g g.lookup0) t
 
 -- Tests
 
 open TokenTree (node)
 
 #guard run
-  Expr.emptyset
+  (Expr.Grammar.singleton Expr.emptyset)
   (node "a" [node "b" [], node "c" [node "d" []]]) =
   Except.ok false
 
 #guard run
-  (Expr.tree (Pred.eq (Token.string "a")) Expr.epsilon)
+  (Expr.Grammar.mk (μ := 2)
+    (Expr.tree (Pred.eq (Token.string "a")) 1)
+    #v[Expr.epsilon]
+  )
   (node "a" []) =
   Except.ok true
 
 #guard run
-  (Expr.tree (Pred.eq (Token.string "a")) Expr.epsilon)
+  (Expr.Grammar.mk (μ := 2)
+    (Expr.tree (Pred.eq (Token.string "a")) 1)
+    #v[Expr.epsilon]
+  )
   (node "a" [node "b" []]) =
   Except.ok false
 
 #guard run
-  (Expr.tree (Pred.eq (Token.string "a"))
-    (Expr.tree (Pred.eq (Token.string "b"))
-      Expr.epsilon
-    )
+  (Expr.Grammar.mk (μ := 3)
+    (Expr.tree (Pred.eq (Token.string "a")) 1)
+    #v[
+      (Expr.tree (Pred.eq (Token.string "b")) 2)
+      , Expr.epsilon
+    ]
   )
-  (node "a" [node "b" []]) =
-  Except.ok true
+  (node "a" [node "b" []])
+  = Except.ok true
 
 #guard run
-  (Expr.tree (Pred.eq (Token.string "a"))
-    (Expr.concat
-      (Expr.tree (Pred.eq (Token.string "b"))
-        Expr.epsilon
+  (Expr.Grammar.mk (μ := 3)
+    (Expr.tree (Pred.eq (Token.string "a")) 1)
+    #v[
+      (Expr.concat
+        (Expr.tree (Pred.eq (Token.string "b")) 2)
+        (Expr.tree (Pred.eq (Token.string "c")) 2)
       )
-      (Expr.tree (Pred.eq (Token.string "c"))
-        Expr.epsilon
-      )
-    )
+      , Expr.epsilon
+    ]
   )
   (node "a" [node "b" [], node "c" []]) =
   Except.ok true
 
 #guard run
-  (Expr.tree (Pred.eq (Token.string "a"))
-    (Expr.concat
-      (Expr.tree (Pred.eq (Token.string "b"))
-        Expr.epsilon
+  (Expr.Grammar.mk (μ := 4)
+    (Expr.tree (Pred.eq (Token.string "a")) 1)
+    #v[
+      (Expr.concat
+        (Expr.tree (Pred.eq (Token.string "b")) 2)
+        (Expr.tree (Pred.eq (Token.string "c")) 3)
       )
-      (Expr.tree (Pred.eq (Token.string "c"))
-        (Expr.tree (Pred.eq (Token.string "d"))
-          Expr.epsilon
-        )
-      )
-    )
+      , Expr.epsilon
+      , (Expr.tree (Pred.eq (Token.string "d")) 2)
+    ]
   )
   (node "a" [node "b" [], node "c" [node "d" []]]) =
   Except.ok true
 
 -- try to engage skip using emptyset, since it is unescapable
 #guard run
-  (Expr.tree (Pred.eq (Token.string "a"))
-    Expr.emptyset
+  (Expr.Grammar.mk (μ := 2)
+    (Expr.tree (Pred.eq (Token.string "a")) 1)
+    #v[Expr.emptyset]
   )
-  (node "a" [node "b" []]) =
-  Except.ok false
+  (node "a" [node "b" []])
+  = Except.ok false
 
 #guard run
-  (Expr.tree (Pred.eq (Token.string "a"))
-    (Expr.concat
-      (Expr.tree (Pred.eq (Token.string "b"))
+  (Expr.Grammar.mk (μ := 5)
+    (Expr.tree (Pred.eq (Token.string "a")) 1)
+    #v[
+      (Expr.concat
+        (Expr.tree (Pred.eq (Token.string "b")) 4)
+        (Expr.tree (Pred.eq (Token.string "c")) 3)
+      )
+      , Expr.epsilon
+      , (Expr.tree (Pred.eq (Token.string "d")) 2)
+      , Expr.emptyset
+    ]
+  )
+  (node "a" [node "b" [], node "c" [node "d" []]])
+  = Except.ok false
+
+#guard run
+  (Expr.Grammar.mk (μ := 3)
+    (Expr.tree (Pred.eq (Token.string "a")) 1)
+    #v[
+      (Expr.concat
+        (Expr.tree (Pred.eq (Token.string "b"))
+          2
+        )
         Expr.emptyset
       )
-      (Expr.tree (Pred.eq (Token.string "c"))
-        (Expr.tree (Pred.eq (Token.string "d"))
-          Expr.epsilon
+      , Expr.epsilon
+    ]
+  )
+  (node "a" [node "b" [], node "c" [node "d" []]]) =
+  Except.ok false
+
+#guard run
+  (Expr.Grammar.mk (μ := 4)
+    (Expr.tree (Pred.eq (Token.string "a")) 1)
+    #v[
+      (Expr.concat
+        (Expr.tree (Pred.eq (Token.string "b"))
+          2
+        )
+        (Expr.tree (Pred.eq (Token.string "c"))
+          3
         )
       )
-    )
+      , Expr.epsilon
+      , Expr.emptyset
+    ]
   )
-  (node "a" [node "b" [], node "c" [node "d" []]]) =
-  Except.ok false
+  (node "a" [node "b" [], node "c" [node "d" []]])
+  = Except.ok false
 
 #guard run
-  (Expr.tree (Pred.eq (Token.string "a"))
-    (Expr.concat
-      (Expr.tree (Pred.eq (Token.string "b"))
-        Expr.epsilon
-      )
-      Expr.emptyset
-    )
-  )
-  (node "a" [node "b" [], node "c" [node "d" []]]) =
-  Except.ok false
-
-#guard run
-  (Expr.tree (Pred.eq (Token.string "a"))
-    (Expr.concat
-      (Expr.tree (Pred.eq (Token.string "b"))
-        Expr.epsilon
-      )
-      (Expr.tree (Pred.eq (Token.string "c"))
-        Expr.emptyset
-      )
-    )
-  )
-  (node "a" [node "b" [], node "c" [node "d" []]]) =
-  Except.ok false
-
-#guard run
-  (Expr.tree (Pred.eq (Token.string "a"))
-    (Expr.concat
-      (Expr.tree (Pred.eq (Token.string "b"))
-        Expr.epsilon
-      )
-      (Expr.tree (Pred.eq (Token.string "c"))
-        (Expr.tree (Pred.eq (Token.string "d"))
-          Expr.emptyset
+  (Expr.Grammar.mk (μ := 5)
+    (Expr.tree (Pred.eq (Token.string "a")) 1)
+    #v[
+      (Expr.concat
+        (Expr.tree (Pred.eq (Token.string "b"))
+          1
+        )
+        (Expr.tree (Pred.eq (Token.string "c"))
+          2
         )
       )
-    )
+      , Expr.epsilon
+      , (Expr.tree (Pred.eq (Token.string "d"))
+          3
+        )
+      , Expr.emptyset
+    ]
   )
-  (node "a" [node "b" [], node "c" [node "d" []]]) =
-  Except.ok false
+  (node "a" [node "b" [], node "c" [node "d" []]])
+  = Except.ok false
