Validator/Memoize/MemLeave.lean
@@ -9,17 +9,17 @@ import Validator.Derive.Leave
 
 namespace MemLeave
 
-abbrev LeaveMap α [DecidableEq α] [Hashable α] := Std.ExtHashMap (Exprs α × List Bool) (Exprs α)
-def LeaveMap.mk [DecidableEq α] [Hashable α]: LeaveMap α := Std.ExtHashMap.emptyWithCapacity
+abbrev LeaveMap μ α [DecidableEq α] [Hashable α] := Std.ExtHashMap (Exprs μ α × List Bool) (Exprs μ α)
+def LeaveMap.mk [DecidableEq α] [Hashable α]: LeaveMap μ α := Std.ExtHashMap.emptyWithCapacity
 
-class MemLeave (m: Type -> Type u) (α: outParam Type) [DecidableEq α] [Hashable α] where
-  getLeave : m (LeaveMap α)
-  setLeave : LeaveMap α → m Unit
+class MemLeave (m: Type -> Type u) (μ: outParam Nat) (α: outParam Type) [DecidableEq α] [Hashable α] where
+  getLeave : m (LeaveMap μ α)
+  setLeave : LeaveMap μ α → m Unit
 
 def deriveLeaveM
   [DecidableEq α] [Hashable α]
-  [Monad m] [Debug m] [MonadExcept String m] [MemLeave m α]
-  (xs: Exprs α) (ns: List Bool): m (Exprs α) := do
+  [Monad m] [Debug m] [MonadExcept String m] [MemLeave m μ α]
+  (xs: Exprs μ α) (ns: List Bool): m (Exprs μ α) := do
   let memoized <- MemLeave.getLeave
   match memoized.get? (xs, ns) with
   | Option.none =>
@@ -31,5 +31,5 @@ def deriveLeaveM
     Debug.debug "cache hit"
     return value
 
-instance [DecidableEq α] [Hashable α] [Monad m] [Debug m] [MonadExcept String m] [MemLeave m α] : Leave.DeriveLeaveM m α where
-  deriveLeaveM (xs: Exprs α) (ns: List Bool): m (Exprs α) := deriveLeaveM xs ns
+instance [DecidableEq α] [Hashable α] [Monad m] [Debug m] [MonadExcept String m] [MemLeave m μ α] : Leave.DeriveLeaveM m μ α where
+  deriveLeaveM (xs: Exprs μ α) (ns: List Bool): m (Exprs μ α) := deriveLeaveM xs ns
