Validator/Validator/Inst/TreeParserMemTestM.lean
@@ -8,32 +8,32 @@ import Validator.Validator.ValidateM
 
 namespace TreeParserMemTestM
 
-structure State (α: Type) [DecidableEq α] [Hashable α] where
+structure State (μ: Nat) (α: Type) [DecidableEq α] [Hashable α] where
   parser: TreeParser.ParserState α
-  enter: MemEnter.EnterMap α
-  leave: MemLeave.LeaveMap α
+  enter: MemEnter.EnterMap μ α
+  leave: MemLeave.LeaveMap μ α
   logs: List String
 
-abbrev Impl (α: Type) [DecidableEq α] [Hashable α] β := EStateM String (State α) β
+abbrev Impl μ (α: Type) [DecidableEq α] [Hashable α] β := EStateM String (State μ α) β
 
-def Impl.mk [DecidableEq α] [Hashable α] (p: TreeParser.ParserState α): State α :=
+def Impl.mk [DecidableEq α] [Hashable α] (p: TreeParser.ParserState α): State μ α :=
   State.mk p MemEnter.EnterMap.mk MemLeave.LeaveMap.mk []
 
-instance [DecidableEq α] [Hashable α]: Debug (Impl α) where
+instance [DecidableEq α] [Hashable α]: Debug (Impl μ α) where
   debug (line: String) := do
     let s <- EStateM.get
     set (State.mk s.parser s.enter s.leave (s.logs ++ [line]))
     return ()
 
-instance [DecidableEq α] [Hashable α]: MonadStateOf (TreeParser.ParserState α) (Impl α) where
-  get : Impl α (TreeParser.ParserState α) := do
+instance [DecidableEq α] [Hashable α]: MonadStateOf (TreeParser.ParserState α) (Impl μ α) where
+  get : Impl μ α (TreeParser.ParserState α) := do
     let s <- EStateM.get
     return s.parser
-  set : TreeParser.ParserState α → Impl α PUnit :=
+  set : TreeParser.ParserState α → Impl μ α PUnit :=
     fun parser => do
       let s <- EStateM.get
       EStateM.set (State.mk parser s.enter s.leave s.logs)
-  modifyGet {β: Type}: (TreeParser.ParserState α → Prod β (TreeParser.ParserState α)) → Impl α β :=
+  modifyGet {β: Type}: (TreeParser.ParserState α → Prod β (TreeParser.ParserState α)) → Impl μ α β :=
     fun f => do
       let s <- EStateM.get
       let (res, parser) := f s.parser
@@ -43,27 +43,27 @@ instance [DecidableEq α] [Hashable α]: MonadStateOf (TreeParser.ParserState α
 instance
   [DecidableEq α]
   [Hashable α]
-  [Monad (Impl α)] -- EStateM is monad
-  [Debug (Impl α)] -- Debug instance is declared above
-  [MonadExcept String (Impl α)] -- EStateM String is MonadExcept String
-  [MonadStateOf (TreeParser.ParserState α) (Impl α)] -- MonadStateOf ParseTree.TreeParser is declared above
-  : Parser (Impl α) α where -- This should just follow, but apparently we need to spell it out
+  [Monad (Impl μ α)] -- EStateM is monad
+  [Debug (Impl μ α)] -- Debug instance is declared above
+  [MonadExcept String (Impl μ α)] -- EStateM String is MonadExcept String
+  [MonadStateOf (TreeParser.ParserState α) (Impl μ α)] -- MonadStateOf ParseTree.TreeParser is declared above
+  : Parser (Impl μ α) α where -- This should just follow, but apparently we need to spell it out
   next := Parser.next
   skip := Parser.skip
   token := Parser.token
 
-instance [DecidableEq α] [Hashable α]: MemEnter.MemEnter (Impl α) α where
-  getEnter : Impl α (MemEnter.EnterMap α) := do
+instance [DecidableEq α] [Hashable α]: MemEnter.MemEnter (Impl μ α) μ α where
+  getEnter : Impl μ α (MemEnter.EnterMap μ α) := do
     let s <- EStateM.get
     return s.enter
-  setEnter : MemEnter.EnterMap α → Impl α PUnit :=
+  setEnter : MemEnter.EnterMap μ α → Impl μ α PUnit :=
     fun enter => do
       let s <- EStateM.get
       set (State.mk s.parser enter s.leave s.logs)
 
 -- This should just follow from the instance declared in MemEnter, but we spell it out just in case.
-instance [DecidableEq α] [Hashable α]: Enter.DeriveEnter (Impl α) α where
-  deriveEnter (xs: Exprs α): Impl α (IfExprs α) := do
+instance [DecidableEq α] [Hashable α]: Enter.DeriveEnter (Impl μ α) μ α where
+  deriveEnter (xs: Exprs μ α): Impl μ α (IfExprs μ α) := do
     let memoized <- MemEnter.MemEnter.getEnter
     match memoized.get? xs with
     | Option.none =>
@@ -72,18 +72,18 @@ instance [DecidableEq α] [Hashable α]: Enter.DeriveEnter (Impl α) α where
       Debug.debug "test cache hit"
       return value
 
-instance [DecidableEq α] [Hashable α]: MemLeave.MemLeave (Impl α) α where
-  getLeave : Impl α (MemLeave.LeaveMap α) := do
+instance [DecidableEq α] [Hashable α]: MemLeave.MemLeave (Impl μ α) μ α where
+  getLeave : Impl μ α (MemLeave.LeaveMap μ α) := do
     let s <- EStateM.get
     return s.leave
-  setLeave : MemLeave.LeaveMap α → Impl α PUnit :=
+  setLeave : MemLeave.LeaveMap μ α → Impl μ α PUnit :=
     fun leave => do
       let s <- EStateM.get
       set (State.mk s.parser s.enter leave s.logs)
 
 -- This should just follow from the instance declared in MemLeave, but we spell it out just in case.
-instance [DecidableEq α] [Hashable α]: Leave.DeriveLeaveM (Impl α) α where
-  deriveLeaveM (xs: Exprs α) (ns: List Bool): Impl α (Exprs α) := do
+instance [DecidableEq α] [Hashable α]: Leave.DeriveLeaveM (Impl μ α) μ α where
+  deriveLeaveM (xs: Exprs μ α) (ns: List Bool): Impl μ α (Exprs μ α) := do
     let memoized <- MemLeave.MemLeave.getLeave
     match memoized.get? (xs, ns) with
     | Option.none =>
@@ -92,17 +92,17 @@ instance [DecidableEq α] [Hashable α]: Leave.DeriveLeaveM (Impl α) α where
       Debug.debug "test cache hit"
       return value
 
-instance [DecidableEq α] [Hashable α]: ValidateM (Impl α) α  where
+instance [DecidableEq α] [Hashable α]: ValidateM (Impl μ α) μ α  where
   -- all instances have been created, so no implementations are required here
 
 def runPopulatedMem
   [DecidableEq α] [Hashable α]
-  (f: Impl α β) (t: ParseTree α) (e: MemEnter.EnterMap α) (l: MemLeave.LeaveMap α): EStateM.Result String (State α) β :=
+  (f: Impl μ α β) (t: ParseTree α) (e: MemEnter.EnterMap μ α) (l: MemLeave.LeaveMap μ α): EStateM.Result String (State μ α) β :=
   EStateM.run f (State.mk (TreeParser.ParserState.mk' t) e l [])
 
 def run'
   [DecidableEq α] [Hashable α]
-  (f: Impl α β) (t: ParseTree α): Except String β :=
+  (f: Impl μ α β) (t: ParseTree α): Except String β :=
   match EStateM.run f (Impl.mk (TreeParser.ParserState.mk' t)) with
   | EStateM.Result.ok k _ => Except.ok k
   | EStateM.Result.error err _ => Except.error err
