Validator/Expr/Compress.lean
@@ -6,7 +6,7 @@ inductive Index where
  | val (n: Nat)
  | emptyset -- emptyset is unescapable, so it gets a special index
 
-def indexOf [DecidableEq α] (xs: Exprs α) (y: (Expr α)): Except String Index :=
+def indexOf [DecidableEq α] (xs: Exprs μ α) (y: (Expr μ α)): Except String Index :=
   match y with
   | Expr.emptyset => Except.ok Index.emptyset
   | _ =>
@@ -14,7 +14,7 @@ def indexOf [DecidableEq α] (xs: Exprs α) (y: (Expr α)): Except String Index 
     | Option.none => Except.error "indexOf: unable to find expression"
     | Option.some idx => Except.ok (Index.val idx)
 
-def ofIndex' (xs: Exprs α) (index: Nat): Except String (Expr α) :=
+def ofIndex' (xs: Exprs μ α) (index: Nat): Except String (Expr μ α) :=
   match xs with
   | [] => Except.error "index overflow"
   | (x::xs') =>
@@ -22,7 +22,7 @@ def ofIndex' (xs: Exprs α) (index: Nat): Except String (Expr α) :=
     | 0 => Except.ok x
     | (n' + 1) => ofIndex' xs' n'
 
-def ofIndex (xs: Exprs α) (index: Index): Except String (Expr α) :=
+def ofIndex (xs: Exprs μ α) (index: Index): Except String (Expr μ α) :=
   match index with
   | Index.emptyset => Except.ok Expr.emptyset
   | Index.val n =>
@@ -35,25 +35,25 @@ inductive Indices where
   | mk (indices: List Index)
 
 -- compress compresses a list of expressions.
-def compress [DecidableEq α] (xs: Exprs α): Except String ((Exprs α) × Indices) := do
+def compress [DecidableEq α] (xs: Exprs μ α): Except String ((Exprs μ α) × Indices) := do
   -- sort to increase chance of cache hit
   -- TODO: let sxs := List.mergeSort xs
   -- remove duplicates
   let sxs' := List.eraseReps xs
   -- remove unescapable expressions, currently only emptyset
-  let sxs'': Exprs α := List.erase sxs' Expr.emptyset
+  let sxs'': Exprs μ α := List.erase sxs' Expr.emptyset
   -- find all indexes of the original expressions in the compressed expressions
   let indexes: List Index <- List.mapM (indexOf sxs'') xs
   return (sxs'', Indices.mk indexes)
 
-def compressM [DecidableEq α] [Monad m] [MonadExcept String m] (xs: Exprs α): m ((Exprs α) × Indices) := do
+def compressM [DecidableEq α] [Monad m] [MonadExcept String m] (xs: Exprs μ α): m ((Exprs μ α) × Indices) := do
   MonadExcept.ofExcept (compress xs)
 
 -- expand expands a list of expressions.
-def expand (indices: Indices) (xs: Exprs α): Except String (Exprs α) :=
+def expand (indices: Indices) (xs: Exprs μ α): Except String (Exprs μ α) :=
   match indices with
   | Indices.mk indexes =>
     List.mapM (ofIndex xs) indexes
 
-def expandM [Monad m] [MonadExcept String m] (indices: Indices) (xs: Exprs α): m (Exprs α) :=
+def expandM [Monad m] [MonadExcept String m] (indices: Indices) (xs: Exprs μ α): m (Exprs μ α) :=
   MonadExcept.ofExcept (expand indices xs)
