Validator/Std/List.lean
@@ -1,6 +1,6 @@
 namespace List
 
-theorem elem_lt_list [SizeOf α] {xs: List α} (h: x ∈ xs): sizeOf x ≤ sizeOf xs := by
+theorem list_elem_lt [SizeOf α] {xs: List α} (h: x ∈ xs): sizeOf x ≤ sizeOf xs := by
   rw [show (x ∈ xs) = List.Mem x xs from rfl] at h
   induction h with
   | head xs' =>
@@ -13,3 +13,12 @@ theorem list_foldl_attach {f: β -> α -> β} {init: β} {xs: List α}:
   List.foldl (fun res ⟨x, _hx⟩ => f res x) init (List.attach xs)
   = List.foldl f init xs := by
   simp only [foldl_subtype, unattach_attach]
+
+theorem list_splitAt_n: xs = (List.splitAt n xs).1 ++ (List.splitAt n xs).2 := by
+  simp only [List.splitAt_eq, List.take_append_drop]
+
+theorem list_splitAt_fst_take: (List.splitAt n xs).1 = take n xs := by
+  simp only [List.splitAt_eq]
+
+theorem list_splitAt_snd_drop: (List.splitAt n xs).2 = drop n xs := by
+  simp only [List.splitAt_eq]
