Validator/Validator/TestIO.lean
@@ -8,14 +8,14 @@ import Validator.Validator.ValidateM
 
 namespace TestIO
 
-def validate {m} [DecidableEq α] [ValidateM m α] (x: Expr α): m Bool :=
-  Validate.validate x
+def validate {m} [DecidableEq α] [ValidateM m μ α] (g: Expr.Grammar μ α) (x: Expr μ α): m Bool :=
+  Validate.validate g x
 
-unsafe def run [DecidableEq α] [Hashable α] (x: Expr α) (t: ParseTree α): Except String Bool :=
-  unsafeEIO (TreeParserIO.run' (validate x) t)
+unsafe def run [DecidableEq α] [Hashable α] (g: Expr.Grammar μ α) (t: ParseTree α): Except String Bool :=
+  unsafeEIO (TreeParserIO.run' (μ := μ) (validate g g.lookup0) t)
 
 -- runTwice is used to check if the cache was hit on the second run
-def runTwice [DecidableEq α] [Hashable α] [DecidableEq β] (f: TreeParserIO.Impl α β) (t: ParseTree α): EIO String β := do
+def runTwice [DecidableEq α] [Hashable α] [DecidableEq β] (f: TreeParserIO.Impl μ α β) (t: ParseTree α): EIO String β := do
   let initial := TreeParserIO.Impl.mk (TreeParser.ParserState.mk' t)
   let (res1, updated) <- StateT.run f initial
   _ <- TreeParserIO.EIO.println "start second run"
@@ -25,116 +25,139 @@ def runTwice [DecidableEq α] [Hashable α] [DecidableEq β] (f: TreeParserIO.Im
   else return res1
 
 -- runTwice is used to check if the cache was hit on the second run
-unsafe def runTwice' [DecidableEq α] [Hashable α] (x: Expr α) (t: ParseTree α): Except String Bool :=
-  unsafeEIO (runTwice (validate x) t)
+unsafe def runTwice' [DecidableEq α] [Hashable α] (g: Expr.Grammar μ α) (t: ParseTree α): Except String Bool :=
+  unsafeEIO (runTwice (μ := μ) (validate g g.lookup0) t)
 
 open TokenTree (node)
 
 -- #eval runTwice'
---   Expr.emptyset
+--   (Expr.Grammar.singleton Expr.emptyset)
 --   (node "a" [node "b" [], node "c" [node "d" []]])
 
 -- #eval runTwice'
---   (Expr.tree (Pred.eq (Token.string "a")) Expr.epsilon)
+--   (Expr.Grammar.mk (μ := 2)
+--     (Expr.tree (Pred.eq (Token.string "a")) 1)
+--     #v[Expr.epsilon]
+--   )
 --   (node "a" [])
 
 -- #eval runTwice'
---   (Expr.tree (Pred.eq (Token.string "a")) Expr.epsilon)
---   (node "a" [node "b" []])
-
--- #eval runTwice'
---   (Expr.tree (Pred.eq (Token.string "a"))
---     (Expr.tree (Pred.eq (Token.string "b"))
---       Expr.epsilon
---     )
+--   (Expr.Grammar.mk (μ := 2)
+--     (Expr.tree (Pred.eq (Token.string "a")) 1)
+--     #v[Expr.epsilon]
 --   )
 --   (node "a" [node "b" []])
 
 -- #eval runTwice'
---   (Expr.tree (Pred.eq (Token.string "a"))
---     (Expr.concat
---       (Expr.tree (Pred.eq (Token.string "b"))
---         Expr.epsilon
+--   (Expr.Grammar.mk (μ := 3)
+--     (Expr.tree (Pred.eq (Token.string "a")) 1)
+--     #v[
+--       (Expr.tree (Pred.eq (Token.string "b")) 2)
+--       , Expr.epsilon
+--     ]
+--   )
+--   (node "a" [node "b" []])
+
+-- #eval runTwice'
+--   (Expr.Grammar.mk (μ := 3)
+--     (Expr.tree (Pred.eq (Token.string "a")) 1)
+--     #v[
+--       (Expr.concat
+--         (Expr.tree (Pred.eq (Token.string "b")) 2)
+--         (Expr.tree (Pred.eq (Token.string "c")) 2)
 --       )
---       (Expr.tree (Pred.eq (Token.string "c"))
---         Expr.epsilon
---       )
---     )
+--       , Expr.epsilon
+--     ]
 --   )
 --   (node "a" [node "b" [], node "c" []])
 
 -- #eval runTwice'
---   (Expr.tree (Pred.eq (Token.string "a"))
---     (Expr.concat
---       (Expr.tree (Pred.eq (Token.string "b"))
---         Expr.epsilon
+--   (Expr.Grammar.mk (μ := 4)
+--     (Expr.tree (Pred.eq (Token.string "a")) 1)
+--     #v[
+--       (Expr.concat
+--         (Expr.tree (Pred.eq (Token.string "b")) 2)
+--         (Expr.tree (Pred.eq (Token.string "c")) 3)
 --       )
---       (Expr.tree (Pred.eq (Token.string "c"))
---         (Expr.tree (Pred.eq (Token.string "d"))
---           Expr.epsilon
---         )
---       )
---     )
+--       , Expr.epsilon
+--       , (Expr.tree (Pred.eq (Token.string "d")) 2)
+--     ]
 --   )
 --   (node "a" [node "b" [], node "c" [node "d" []]])
 
 -- -- try to engage skip using emptyset, since it is unescapable
 -- #eval runTwice'
---   (Expr.tree (Pred.eq (Token.string "a"))
---     Expr.emptyset
+--   (Expr.Grammar.mk (μ := 2)
+--     (Expr.tree (Pred.eq (Token.string "a")) 1)
+--     #v[Expr.emptyset]
 --   )
 --   (node "a" [node "b" []])
 
 -- #eval runTwice'
---   (Expr.tree (Pred.eq (Token.string "a"))
---     (Expr.concat
---       (Expr.tree (Pred.eq (Token.string "b"))
+--   (Expr.Grammar.mk (μ := 5)
+--     (Expr.tree (Pred.eq (Token.string "a")) 1)
+--     #v[
+--       (Expr.concat
+--         (Expr.tree (Pred.eq (Token.string "b")) 4)
+--         (Expr.tree (Pred.eq (Token.string "c")) 3)
+--       )
+--       , Expr.epsilon
+--       , (Expr.tree (Pred.eq (Token.string "d")) 2)
+--       , Expr.emptyset
+--     ]
+--   )
+--   (node "a" [node "b" [], node "c" [node "d" []]])
+
+-- #eval runTwice'
+--   (Expr.Grammar.mk (μ := 3)
+--     (Expr.tree (Pred.eq (Token.string "a")) 1)
+--     #v[
+--       (Expr.concat
+--         (Expr.tree (Pred.eq (Token.string "b"))
+--           2
+--         )
 --         Expr.emptyset
 --       )
---       (Expr.tree (Pred.eq (Token.string "c"))
---         (Expr.tree (Pred.eq (Token.string "d"))
---           Expr.epsilon
+--       , Expr.epsilon
+--     ]
+--   )
+--   (node "a" [node "b" [], node "c" [node "d" []]])
+
+-- #eval runTwice'
+--   (Expr.Grammar.mk (μ := 4)
+--     (Expr.tree (Pred.eq (Token.string "a")) 1)
+--     #v[
+--       (Expr.concat
+--         (Expr.tree (Pred.eq (Token.string "b"))
+--           2
+--         )
+--         (Expr.tree (Pred.eq (Token.string "c"))
+--           3
 --         )
 --       )
---     )
+--       , Expr.epsilon
+--       , Expr.emptyset
+--     ]
 --   )
 --   (node "a" [node "b" [], node "c" [node "d" []]])
 
--- #eval runTwice'
---   (Expr.tree (Pred.eq (Token.string "a"))
---     (Expr.concat
---       (Expr.tree (Pred.eq (Token.string "b"))
---         Expr.epsilon
---       )
---       Expr.emptyset
---     )
---   )
---   (node "a" [node "b" [], node "c" [node "d" []]])
-
--- #eval runTwice'
---   (Expr.tree (Pred.eq (Token.string "a"))
---     (Expr.concat
---       (Expr.tree (Pred.eq (Token.string "b"))
---         Expr.epsilon
---       )
---       (Expr.tree (Pred.eq (Token.string "c"))
---         Expr.emptyset
---       )
---     )
---   )
---   (node "a" [node "b" [], node "c" [node "d" []]])
-
--- #eval runTwice'
---   (Expr.tree (Pred.eq (Token.string "a"))
---     (Expr.concat
---       (Expr.tree (Pred.eq (Token.string "b"))
---         Expr.epsilon
---       )
---       (Expr.tree (Pred.eq (Token.string "c"))
---         (Expr.tree (Pred.eq (Token.string "d"))
---           Expr.emptyset
+--  #eval runTwice'
+--    (Expr.Grammar.mk (μ := 5)
+--     (Expr.tree (Pred.eq (Token.string "a")) 1)
+--     #v[
+--       (Expr.concat
+--         (Expr.tree (Pred.eq (Token.string "b"))
+--           1
+--         )
+--         (Expr.tree (Pred.eq (Token.string "c"))
+--           2
 --         )
 --       )
---     )
+--       , Expr.epsilon
+--       , (Expr.tree (Pred.eq (Token.string "d"))
+--           3
+--         )
+--       , Expr.emptyset
+--     ]
 --   )
 --   (node "a" [node "b" [], node "c" [node "d" []]])
