Validator/Validator/TestMem.lean
@@ -8,21 +8,21 @@ import Validator.Validator.Inst.TreeParserMemTestM
 
 namespace TestMem
 
-def validate {m} [DecidableEq α] [ValidateM m α] (x: Expr α): m Bool :=
-  Validate.validate x
+def validate {m} [DecidableEq α] [ValidateM m μ α] (g: Expr.Grammar μ α) (x: Expr μ α): m Bool :=
+  Validate.validate g x
 
-def run [DecidableEq α] [Hashable α] (x: Expr α) (t: ParseTree α): Except String Bool :=
-  TreeParserMemM.run' (validate x) t
+def run [DecidableEq α] [Hashable α] (g: Expr.Grammar μ α) (t: ParseTree α): Except String Bool :=
+  TreeParserMemM.run' (μ := μ) (validate g g.lookup0) t
 
 -- Tests
 
 def testCacheIsHitOnSecondRun
   [DecidableEq α] [Hashable α]
-  (x: Expr α) (t: ParseTree α): Except String Bool :=
-  match TreeParserMemM.run (validate x) t with
+  (g: Expr.Grammar μ α) (t: ParseTree α): Except String Bool :=
+  match TreeParserMemM.run (μ := μ) (validate g g.lookup0) t with
   | EStateM.Result.error err _ => Except.error err
   | EStateM.Result.ok res1 state =>
-    match TreeParserMemTestM.runPopulatedMem (validate x) t state.enter state.leave with
+    match TreeParserMemTestM.runPopulatedMem (μ := μ) (validate g g.lookup0) t state.enter state.leave with
     | EStateM.Result.error err _ => Except.error err
     | EStateM.Result.ok res2 _ =>
       if res1 ≠ res2
@@ -33,132 +33,161 @@ def testCacheIsHitOnSecondRun
 -- This tests that given an empty cache the test does actually fail.
 def testThatTestCacheBreaksWithEmptyCache
   [DecidableEq α] [Hashable α]
-  (x: Expr α) (t: ParseTree α): Except String Bool :=
-  TreeParserMemTestM.run' (validate x) t
+  (g: Expr.Grammar μ α) (t: ParseTree α): Except String Bool :=
+  TreeParserMemTestM.run' (μ := μ) (validate g g.lookup0) t
 
 open TokenTree (node)
 
 #guard testCacheIsHitOnSecondRun
-  Expr.emptyset
-  (node "a" [node "b" [], node "c" [node "d" []]]) =
-  Except.ok false
+  (Expr.Grammar.mk (μ := 2)
+    (Expr.tree (Pred.eq (Token.string "a")) 1)
+    #v[Expr.epsilon]
+  )
+  (node "a" [node "b" [], node "c" [node "d" []]])
+  = Except.ok false
 
 #guard testCacheIsHitOnSecondRun
-  (Expr.tree (Pred.eq (Token.string "a")) Expr.epsilon)
-  (node "a" []) =
-  Except.ok true
+  (Expr.Grammar.mk (μ := 2)
+    (Expr.tree (Pred.eq (Token.string "a")) 1)
+    #v[Expr.epsilon]
+  )
+  (node "a" [])
+  = Except.ok true
 
 #guard testThatTestCacheBreaksWithEmptyCache
-  (Expr.tree (Pred.eq (Token.string "a")) Expr.epsilon)
-  (node "a" []) =
-  Except.error "test cache miss"
-
-#guard testCacheIsHitOnSecondRun
-  (Expr.tree (Pred.eq (Token.string "a")) Expr.epsilon)
-  (node "a" [node "b" []]) =
-  Except.ok false
-
-#guard testCacheIsHitOnSecondRun
-  (Expr.tree (Pred.eq (Token.string "a"))
-    (Expr.tree (Pred.eq (Token.string "b"))
-      Expr.epsilon
-    )
+  (Expr.Grammar.mk (μ := 2)
+    (Expr.tree (Pred.eq (Token.string "a")) 1)
+    #v[Expr.epsilon]
   )
-  (node "a" [node "b" []]) =
-  Except.ok true
+  (node "a" [])
+  = Except.error "test cache miss"
 
 #guard testCacheIsHitOnSecondRun
-  (Expr.tree (Pred.eq (Token.string "a"))
-    (Expr.concat
-      (Expr.tree (Pred.eq (Token.string "b"))
-        Expr.epsilon
-      )
-      (Expr.tree (Pred.eq (Token.string "c"))
-        Expr.epsilon
-      )
-    )
+  (Expr.Grammar.mk (μ := 2)
+    (Expr.tree (Pred.eq (Token.string "a")) 1)
+    #v[Expr.epsilon]
   )
-  (node "a" [node "b" [], node "c" []]) =
-  Except.ok true
+  (node "a" [node "b" []])
+  = Except.ok false
 
 #guard testCacheIsHitOnSecondRun
-  (Expr.tree (Pred.eq (Token.string "a"))
-    (Expr.concat
-      (Expr.tree (Pred.eq (Token.string "b"))
-        Expr.epsilon
-      )
-      (Expr.tree (Pred.eq (Token.string "c"))
-        (Expr.tree (Pred.eq (Token.string "d"))
-          Expr.epsilon
-        )
-      )
-    )
+  (Expr.Grammar.mk (μ := 3)
+    (Expr.tree (Pred.eq (Token.string "a")) 1)
+    #v[
+      (Expr.tree (Pred.eq (Token.string "b")) 2)
+      , Expr.epsilon
+    ]
   )
-  (node "a" [node "b" [], node "c" [node "d" []]]) =
-  Except.ok true
+  (node "a" [node "b" []])
+  = Except.ok true
+
+#guard testCacheIsHitOnSecondRun
+  (Expr.Grammar.mk (μ := 3)
+    (Expr.tree (Pred.eq (Token.string "a")) 1)
+    #v[
+      (Expr.concat
+        (Expr.tree (Pred.eq (Token.string "b")) 2)
+        (Expr.tree (Pred.eq (Token.string "c")) 2)
+      )
+      , Expr.epsilon
+    ]
+  )
+  (node "a" [node "b" [], node "c" []])
+  = Except.ok true
+
+#guard testCacheIsHitOnSecondRun
+  (Expr.Grammar.mk (μ := 4)
+    (Expr.tree (Pred.eq (Token.string "a")) 1)
+    #v[
+      (Expr.concat
+        (Expr.tree (Pred.eq (Token.string "b")) 2)
+        (Expr.tree (Pred.eq (Token.string "c")) 3)
+      )
+      , Expr.epsilon
+      , (Expr.tree (Pred.eq (Token.string "d")) 2)
+    ]
+  )
+  (node "a" [node "b" [], node "c" [node "d" []]])
+  = Except.ok true
 
 -- try to engage skip using emptyset, since it is unescapable
 #guard testCacheIsHitOnSecondRun
-  (Expr.tree (Pred.eq (Token.string "a"))
-    Expr.emptyset
+  (Expr.Grammar.mk (μ := 2)
+    (Expr.tree (Pred.eq (Token.string "a")) 1)
+    #v[Expr.emptyset]
   )
   (node "a" [node "b" []]) =
   Except.ok false
 
 #guard testCacheIsHitOnSecondRun
-  (Expr.tree (Pred.eq (Token.string "a"))
-    (Expr.concat
-      (Expr.tree (Pred.eq (Token.string "b"))
+  (Expr.Grammar.mk (μ := 5)
+    (Expr.tree (Pred.eq (Token.string "a")) 1)
+    #v[
+      (Expr.concat
+        (Expr.tree (Pred.eq (Token.string "b")) 4)
+        (Expr.tree (Pred.eq (Token.string "c")) 3)
+      )
+      , Expr.epsilon
+      , (Expr.tree (Pred.eq (Token.string "d")) 2)
+      , Expr.emptyset
+    ]
+  )
+  (node "a" [node "b" [], node "c" [node "d" []]]) =
+  Except.ok false
+
+#guard testCacheIsHitOnSecondRun
+  (Expr.Grammar.mk (μ := 3)
+    (Expr.tree (Pred.eq (Token.string "a")) 1)
+    #v[
+      (Expr.concat
+        (Expr.tree (Pred.eq (Token.string "b"))
+          2
+        )
         Expr.emptyset
       )
-      (Expr.tree (Pred.eq (Token.string "c"))
-        (Expr.tree (Pred.eq (Token.string "d"))
-          Expr.epsilon
+      , Expr.epsilon
+    ]
+  )
+  (node "a" [node "b" [], node "c" [node "d" []]]) =
+  Except.ok false
+
+#guard testCacheIsHitOnSecondRun
+  (Expr.Grammar.mk (μ := 4)
+    (Expr.tree (Pred.eq (Token.string "a")) 1)
+    #v[
+      (Expr.concat
+        (Expr.tree (Pred.eq (Token.string "b"))
+          2
+        )
+        (Expr.tree (Pred.eq (Token.string "c"))
+          3
         )
       )
-    )
+      , Expr.epsilon
+      , Expr.emptyset
+    ]
   )
   (node "a" [node "b" [], node "c" [node "d" []]]) =
   Except.ok false
 
 #guard testCacheIsHitOnSecondRun
-  (Expr.tree (Pred.eq (Token.string "a"))
-    (Expr.concat
-      (Expr.tree (Pred.eq (Token.string "b"))
-        Expr.epsilon
-      )
-      Expr.emptyset
-    )
-  )
-  (node "a" [node "b" [], node "c" [node "d" []]]) =
-  Except.ok false
-
-#guard testCacheIsHitOnSecondRun
-  (Expr.tree (Pred.eq (Token.string "a"))
-    (Expr.concat
-      (Expr.tree (Pred.eq (Token.string "b"))
-        Expr.epsilon
-      )
-      (Expr.tree (Pred.eq (Token.string "c"))
-        Expr.emptyset
-      )
-    )
-  )
-  (node "a" [node "b" [], node "c" [node "d" []]]) =
-  Except.ok false
-
-#guard testCacheIsHitOnSecondRun
-  (Expr.tree (Pred.eq (Token.string "a"))
-    (Expr.concat
-      (Expr.tree (Pred.eq (Token.string "b"))
-        Expr.epsilon
-      )
-      (Expr.tree (Pred.eq (Token.string "c"))
-        (Expr.tree (Pred.eq (Token.string "d"))
-          Expr.emptyset
+  (Expr.Grammar.mk (μ := 5)
+    (Expr.tree (Pred.eq (Token.string "a")) 1)
+    #v[
+      (Expr.concat
+        (Expr.tree (Pred.eq (Token.string "b"))
+          1
+        )
+        (Expr.tree (Pred.eq (Token.string "c"))
+          2
         )
       )
-    )
+      , Expr.epsilon
+      , (Expr.tree (Pred.eq (Token.string "d"))
+          3
+        )
+      , Expr.emptyset
+    ]
   )
   (node "a" [node "b" [], node "c" [node "d" []]]) =
   Except.ok false
